Shenzhen/Conns.lean
@@ -5,18 +5,30 @@ import Batteries.Data.List.Basic
 
 public section
 
-structure Conns (nChips : ℕ) (pinType : Type) where
+structure Conns.Node (nChips : ℕ) (nPins : Fin nChips → ℕ) where
+  /-- Which chip -/
+  i : Fin nChips
+  /-- Which pin on chip `i` -/
+  j : Fin (nPins i)
+deriving BEq
+
+structure Conns (nChips : ℕ) (nPins : Fin nChips → ℕ) where
   private mk ::
-  /-- Are two nodes connected? -/
-  connected : (Fin nChips × pinType) → (Fin nChips × pinType) → Bool
+  /-- Are two pins connected? -/
+  connected : Conns.Node nChips nPins → Conns.Node nChips nPins → Bool
 
 namespace Conns
 
+variable {nChips : ℕ} {nPins : Fin nChips → ℕ}
+
 /-- All neighbors of a node, as a list -/
-def neighbors {n m} (conns : Conns n (Fin m)) (i : Fin n) (j : Fin m) : List (Fin n × Fin m) :=
-  (List.finRange n).product (List.finRange m)|>.filter (conns.connected (i, j))
+def neighbors (conns : Conns nChips nPins) : Node nChips nPins → List (Node nChips nPins) := fun v =>
+  (List.finRange nChips).flatMap fun i' =>
+    (List.finRange (nPins i'))
+      |>.map (fun j' => ⟨i', j'⟩)
+      |>.filter (conns.connected v)
 
 /-- Create a `Conns` out of a list of (undirected) edges. This function does *not*
   compute the transitive closure. -/
-def ofEdges [BEq pinType] (edges : List ((Fin nChips × pinType) × (Fin nChips × pinType))) : Conns nChips pinType where
+def ofEdges (edges : List (Node nChips nPins × Node nChips nPins)) : Conns nChips nPins where
   connected u v := edges.contains (u, v) || edges.contains (v, u)
